Reduced words.

Free_Group.thy
@@ -2,9 +2,9 @@ theory Free_Group
 imports Main 
 begin
 
-datatype 'a gentype = C 'a | InvG 'a 
+datatype 'a gentype = C 'a | InvG 'a
 
-primrec inverse :: " 'a gentype \<Rightarrow> 'a gentype"
+primrec inverse :: " 'a gentype ⇒ 'a gentype"
   where
 "inverse (C x) = InvG x"
 |"inverse (InvG x) = C x"
@@ -16,40 +16,44 @@ primrec genset :: "('a gentype) list ⇒ ('a gentype) list"
 
 type_synonym 'a word = "('a gentype) list"
 
-inductive_set spanset :: "('a gentype list) ⇒('a gentype ⇒ 'a gentype ⇒ 'a gentype) ⇒ ('a gentype) set"
+inductive_set spanset :: "('a gentype list) ⇒('a gentype ⇒ 'a gentype ⇒ 'a gentype) ⇒ ('a gentype) list"
   for S :: "('a gentype) list" and f :: "('a gentype⇒ 'a gentype⇒ 'a gentype)" 
   where
 "x ∈ genset S ⟹ x ∈ spanset S f"
 |"x ∈ spanset S f ⟹ y ∈ spanset S f ⟹ (f x y) ∈ spanset S f"
 
-fun is_inverse :: "'a word \<Rightarrow> bool"
+fun is_inverse :: "'a word ⇒ bool"
   where
 "is_inverse [] = False"
 |"is_inverse (x#[]) = False"
 |"is_inverse (x#[y]) = (if x = inverse y then True else False)"
 
-fun reduce :: "'a word \<Rightarrow> 'a word"
+
+fun reduce :: "'a word ⇒ 'a word"
   where
 "reduce [] = []"
 |"reduce (x#[]) = (x#[])"
-|"reduce (x#(y#xys)) = (if is_inverse (x#[y]) then reduce xys else reduce(x#(reduce(y#xys)))"
+|"reduce (x#(y#xys)) = (if is_inverse (x#[y]) then reduce xys else x#(reduce(y#xys)))"
 
-fun is_reduced :: "'a word \<Rightarrow> bool"
+fun is_reduced :: "'a word ⇒ bool"
   where
 "is_reduced [] = True"
 |"is_reduced (x#[]) = True"
 |"is_reduced (x#(y#xys)) = (if is_inverse (x#[y]) then False else is_reduced (y#xys))"
 
+(*define reduced:: "'a gentype set" as a spanset S where ∄ x ∈ S. (y = inverse x) ∈ S"
+ and prove lemma empty_list_is_reduced and set with one element is reduced.*)
+
 (*lemma spanset_prop:
-  assumes "x \<in> spanset n f " 
-  shows "(\<exists> ls. length ls = n) "
+  assumes "x ∈ spanset n f " 
+  shows "(∃ ls. length ls = n) "
 proof-
   using assms by (solve_direct: List.Ex_list_of_length)
 qed 
 
 lemma spanset_prop1:
-  assumes "x \<in> spanset n f " 
-  shows "\<exists> ls. ls = x"
+  assumes "x ∈ spanset n f " 
+  shows "∃ ls. ls = x"
 proof -
   using assms by (solve_direct :  SMT.smt_arith_simplify(45))
 qed 
